MECMAR/spec/base/Numeric.v
@@ -1,6 +1,9 @@
 From Coq Require Import ZArith Lia.
 From Warblre Require Import Result.
 
+Import Result.Notations.
+Local Open Scope result_flow.
+
 (* 5.2.5 Mathematical Operations
    «  Mathematical values: Arbitrary real numbers, used as the default numeric type. »
    «  When the term integer is used in this specification, it refers to a mathematical 
@@ -11,23 +14,51 @@ From Warblre Require Import Result.
 *)
 Definition integer := Z.
 Definition non_neg_integer := nat.
-Definition positive_integer := { n: non_neg_integer | (0 < n)%nat }.
+Definition positive_integer := positive.
 Definition nat_to_nni (n: nat): non_neg_integer := n.
-Definition positive_to_non_neg (n: positive_integer): non_neg_integer := proj1_sig n.
-Definition positive_to_nat (n: positive_integer): nat := proj1_sig n.
+Definition positive_to_non_neg (n: positive_integer): non_neg_integer := Pos.to_nat n.
+Definition positive_to_nat (n: positive_integer): nat := Pos.to_nat n.
 
 Module NonNegInt.
-  Definition to_positive {F: Type} {_: Result.AssertionError F} (n: non_neg_integer): Result positive_integer F.
-    destruct n eqn:Eq_n.
-    - apply Result.assertion_failed.
-    - refine (Success (exist _ n _)). subst. apply Nat.lt_0_succ.
-  Defined.
+  Lemma pos: forall p, positive_to_non_neg p > 0.
+  Proof. intros. pose proof (Pos2Nat.is_pos p). unfold positive_to_non_neg. lia. Qed.
 
-  Lemma to_positive_soundness {F: Type} {_: Result.AssertionError F}: forall n p, to_positive n = Success p -> proj1_sig p = n.
-  Proof. intros. destruct n; cbn in *. - Result.assertion_failed_helper. - injection H as <-. reflexivity. Qed.
+  Fixpoint to_positive {F: Type} {_: Result.AssertionError F} (n: non_neg_integer): Result positive_integer F :=
+     match n with
+       | 0 => Result.assertion_failed
+       | 1 => Success (1%positive)
+       | S x => let! n' =<< to_positive x in Success (Pos.succ n')
+     end.
+
+  Lemma succ {F: Type} {_: Result.AssertionError F}: forall n p, to_positive n = Success p -> to_positive (S n) = Success (Pos.succ p).
+  Proof. intros. cbn in *. destruct n. - Result.assertion_failed_helper. - rewrite -> H. reflexivity. Qed.
+
+  Lemma succ_inv {F: Type} {_: Result.AssertionError F}: forall n p, to_positive (S (S n)) = Success (Pos.succ p) -> to_positive (S n) = Success p.
+  Proof. intros. cbn in *. match goal with | [ |- ?t = _ ] => destruct t end. - injection H as ->%Pos.succ_inj. reflexivity. - discriminate. Qed.
+
+  Lemma to_positive_soundness {F: Type} {_: Result.AssertionError F}: forall n p, to_positive n = Success p -> positive_to_non_neg p = n.
+  Proof.
+    induction n; intros; cbn in *.
+    - Result.assertion_failed_helper. 
+    - destruct n.
+      + injection H as <-. reflexivity.
+      + destruct (to_positive (S n)).
+        * injection H as <-. subst. specialize IHn with (1 := eq_refl).
+          unfold positive_to_non_neg. rewrite -> Pos2Nat.inj_succ. f_equal. assumption.
+        * discriminate.
+  Qed.
 
   Lemma to_positive_completeness {F: Type} {_: Result.AssertionError F}: forall n, 0 < n -> exists p, to_positive n = Success p.
-  Proof. intros. destruct n. - lia. - cbn. eexists. reflexivity. Qed.
+  Proof.
+    induction n; intros.
+    - lia.
+    - destruct n.
+      + exists 1%positive. reflexivity.
+      + specialize (IHn ltac:(lia)) as [ p Eq_p ]. exists (Pos.succ p). apply succ. assumption.
+  Qed.
+
+  Lemma failure {F: Type} {_: Result.AssertionError F}: forall n f, to_positive n = Failure f -> n = 0.
+  Proof. intros. destruct n eqn:Eq_n. - reflexivity. - pose proof (to_positive_completeness (S n0) ltac:(lia)) as [ ? ? ]. congruence. Qed.
 End NonNegInt.
 
 
