MECMAR/spec/StaticSemantics.v
@@ -45,49 +45,34 @@ Module StaticSemantics.
     + rewrite <- IHr with (1 := H). cbn. reflexivity.
   Qed.
 
-  (** 22.2.1.1 Static Semantics: Early Errors *)
+  (** 22.2.1.9 Static Semantics: RegExpIdentifierCodePoints *)
 
-  (** 22.2.1.2 Static Semantics: CountLeftCapturingParensWithin *)
-  Fixpoint countLeftCapturingParensWithin_impl (r: Regex): non_neg_integer :=
-    match r with
-    | Empty => 0
-    | Char _ => 0
-    | Dot => 0
-    | AtomEsc _ => 0
-    | CharacterClass _ => 0
-    | Disjunction r1 r2 => (countLeftCapturingParensWithin_impl r1) + (countLeftCapturingParensWithin_impl r2)
-    | Quantified r0 _ => countLeftCapturingParensWithin_impl r0
-    | Seq r1 r2 => (countLeftCapturingParensWithin_impl r1) + (countLeftCapturingParensWithin_impl r2)
-    | Group _ r0 => 1 + (countLeftCapturingParensWithin_impl r0)
-    | Lookahead r0 => countLeftCapturingParensWithin_impl r0
-    | NegativeLookahead r0 => countLeftCapturingParensWithin_impl r0
-    | Lookbehind r0 => countLeftCapturingParensWithin_impl r0
-    | NegativeLookbehind r0 => countLeftCapturingParensWithin_impl r0
-    end.
-  Definition countLeftCapturingParensWithin (r: Regex) (ctx: RegexContext): non_neg_integer := countLeftCapturingParensWithin_impl r.
+  (** 22.2.1.10 Static Semantics: RegExpIdentifierCodePoint *)
 
-  (** 22.2.1.3 Static Semantics: CountLeftCapturingParensBefore *)
-  Fixpoint countLeftCapturingParensBefore_impl (ctx: RegexContext): non_neg_integer :=
-    match ctx with
-    | nil => 0
-    | h :: t => (countLeftCapturingParensBefore_impl t) + match h with
-      | Disjunction_left _ => 0
-      | Disjunction_right l => countLeftCapturingParensWithin_impl l
-      | Quantified_inner _ => 0
-      | Seq_left _ => 0
-      | Seq_right l => countLeftCapturingParensWithin_impl l
-      | Group_inner _ => 1
-      | Lookahead_inner => 0
-      | NegativeLookahead_inner => 0
-      | Lookbehind_inner => 0
-      | NegativeLookbehind_inner => 0
+  (** 22.2.1.8 Static Semantics: CapturingGroupName *)
+  Definition capturingGroupName (gn: GroupName): GroupName := gn.
+
+  (** 22.2.1.7 Static Semantics: GroupSpecifiersThatMatch ( thisGroupName ) *)
+  Definition groupSpecifiersThatMatch (r: Regex) (ctx: RegexContext) (thisGroupName: GroupName): list (Regex * RegexContext) :=
+    (* 1. Let name be the CapturingGroupName of thisGroupName. *)
+    let name := capturingGroupName thisGroupName in
+    (* 2. Let pattern be the Pattern containing thisGroupName. *)
+    let pattern := zip r ctx in
+    (* 3. Let result be a new empty List. *)
+    (* 4. For each GroupSpecifier gs that pattern contains, do *)
+    let result := List.flat_map ( fun r => match r with
+      | (Group (Some gs) inner, ctx) =>
+        (* a. If the CapturingGroupName of gs is name, then *)
+        if (GroupName.eqs gs name) then
+          (* i. Append gs to result. *)
+          (inner, Group_inner (Some gs) :: ctx) :: nil
+        else nil
+      | _ => nil
       end
-    end.
-  Definition countLeftCapturingParensBefore (r: Regex) (ctx: RegexContext): non_neg_integer := countLeftCapturingParensBefore_impl ctx.
-
-  (** 22.2.1.4 Static Semantics: CapturingGroupNumber *)
-
-  (** 22.2.1.5 Static Semantics: IsCharacterClass *)
+      ) (pre_order_walk pattern nil)
+    in
+    (* 5. Return result. *)
+    result.
 
   (** 22.2.1.6 Static Semantics: CharacterValue *)
   Definition characterValue {F: Type} {_: Result.AssertionError F} (self: ClassAtom): Result non_neg_integer F := match self with
@@ -135,32 +120,68 @@ Module StaticSemantics.
   | _ => Result.assertion_failed
   end.
 
-  (** 22.2.1.7 Static Semantics: GroupSpecifiersThatMatch ( thisGroupName ) *)
-  Definition groupSpecifiersThatMatch (r: Regex) (ctx: RegexContext) (thisGroupName: GroupName): list (Regex * RegexContext) :=
-    (* 1. Let name be the CapturingGroupName of thisGroupName. *)
-    let name := thisGroupName in
-    (* 2. Let pattern be the Pattern containing thisGroupName. *)
-    let pattern := zip r ctx in
-    (* 3. Let result be a new empty List. *)
-    (* 4. For each GroupSpecifier gs that pattern contains, do *)
-    let result := List.flat_map ( fun r => match r with
-      | (Group (Some gs) inner, ctx) =>
-        (* a. If the CapturingGroupName of gs is name, then *)
-        if (GroupName.eqs gs name) then
-          (* i. Append gs to result. *)
-          (inner, Group_inner (Some gs) :: ctx) :: nil
-        else nil
-      | _ => nil
+  (** 22.2.1.5 Static Semantics: IsCharacterClass *)
+
+  (** 22.2.1.4 Static Semantics: CapturingGroupNumber *)
+
+  (** 22.2.1.2 Static Semantics: CountLeftCapturingParensWithin *)
+  Fixpoint countLeftCapturingParensWithin_impl (r: Regex): non_neg_integer :=
+    match r with
+    | Empty => 0
+    | Char _ => 0
+    | Dot => 0
+    | AtomEsc _ => 0
+    | CharacterClass _ => 0
+    | Disjunction r1 r2 => (countLeftCapturingParensWithin_impl r1) + (countLeftCapturingParensWithin_impl r2)
+    | Quantified r0 _ => countLeftCapturingParensWithin_impl r0
+    | Seq r1 r2 => (countLeftCapturingParensWithin_impl r1) + (countLeftCapturingParensWithin_impl r2)
+    | Group _ r0 => 1 + (countLeftCapturingParensWithin_impl r0)
+    | Lookahead r0 => countLeftCapturingParensWithin_impl r0
+    | NegativeLookahead r0 => countLeftCapturingParensWithin_impl r0
+    | Lookbehind r0 => countLeftCapturingParensWithin_impl r0
+    | NegativeLookbehind r0 => countLeftCapturingParensWithin_impl r0
+    end.
+  Definition countLeftCapturingParensWithin (r: Regex) (ctx: RegexContext): non_neg_integer := countLeftCapturingParensWithin_impl r.
+
+  (** 22.2.1.3 Static Semantics: CountLeftCapturingParensBefore *)
+  Fixpoint countLeftCapturingParensBefore_impl (ctx: RegexContext): non_neg_integer :=
+    match ctx with
+    | nil => 0
+    | h :: t => (countLeftCapturingParensBefore_impl t) + match h with
+      | Disjunction_left _ => 0
+      | Disjunction_right l => countLeftCapturingParensWithin_impl l
+      | Quantified_inner _ => 0
+      | Seq_left _ => 0
+      | Seq_right l => countLeftCapturingParensWithin_impl l
+      | Group_inner _ => 1
+      | Lookahead_inner => 0
+      | NegativeLookahead_inner => 0
+      | Lookbehind_inner => 0
+      | NegativeLookbehind_inner => 0
       end
-      ) (pre_order_walk pattern nil)
-    in
-    (* 5. Return result. *)
-    result.
+    end.
+  Definition countLeftCapturingParensBefore (r: Regex) (ctx: RegexContext): non_neg_integer := countLeftCapturingParensBefore_impl ctx.
 
-  (** 22.2.1.8 Static Semantics: CapturingGroupName *)
-
-  (** 22.2.1.9 Static Semantics: RegExpIdentifierCodePoints *)
-
-  (** 22.2.1.10 Static Semantics: RegExpIdentifierCodePoint *)
+  (** 22.2.1.1 Static Semantics: Early Errors *)
+  (*Definition earlyErrors (r: Regex): bool :=
+    let nodes := pre_order_walk r nil in
+    (**  Pattern :: Disjunction *)
+    (* * It is a Syntax Error if CountLeftCapturingParensWithin(Pattern) ≥ 2^32 - 1. *)
+    (* if (countLeftCapturingParensWithin r nil >=? 4294967295)%nat then true *)
+    (* * It is a Syntax Error if Pattern contains two or more GroupSpecifiers for which CapturingGroupName of GroupSpecifier is the same. *)
+    if List.Exists.exists nodes (fun node0 =>
+      List.Exists.exists nodes (fun node1 =>
+        
+    )) then true
+    (**  QuantifierPrefix :: { DecimalDigits , DecimalDigits } *)
+    (* * It is a Syntax Error if the MV of the first DecimalDigits is strictly greater than the MV of the second DecimalDigits. *)
+    (**  AtomEscape :: k GroupName *)
+    (* * It is a Syntax Error if GroupSpecifiersThatMatch(GroupName) is empty. *)
+    (**  AtomEscape :: DecimalEscape *)
+    (* * It is a Syntax Error if the CapturingGroupNumber of DecimalEscape is strictly greater than CountLeftCapturingParensWithin(the Pattern containing AtomEscape). *)
+    (**  NonemptyClassRanges :: ClassAtom - ClassAtom ClassRanges *)
+    (* * It is a Syntax Error if IsCharacterClass of the first ClassAtom is true or IsCharacterClass of the second ClassAtom is true. *)
+    (* It is a Syntax Error if IsCharacterClass of the first ClassAtom is false, IsCharacterClass of the second ClassAtom is false, and the CharacterValue of the first ClassAtom is strictly greater than the CharacterValue of the second ClassAtom.  *)
+    else false.*)
 End StaticSemantics.
 Export StaticSemantics.
